src/sequential/NoMix.v
@@ -1,0 +1,39 @@
+From sflib Require Import sflib.
+From Paco Require Import paco.
+
+From PromisingLib Require Import Axioms.
+From PromisingLib Require Import Basic.
+From PromisingLib Require Import Loc.
+From PromisingLib Require Import Language.
+Require Import Simple.
+
+Require Import Event.
+
+Section NOMIX.
+  Variable loc_na: Loc.t -> Prop.
+  Variable loc_at: Loc.t -> Prop.
+
+  Definition _nomix
+             (nomix: forall (lang: language) (st: lang.(Language.state)), Prop)
+             (lang: language) (st: lang.(Language.state)): Prop :=
+    forall st1 e
+           (STEP: lang.(Language.step) e st st1),
+      (<<NA: forall l c (NA: is_atomic_event e = false) (ACC: is_accessing e = Some (l, c)), loc_na l>>) /\
+        (<<AT: forall l c (AT: is_atomic_event e = true) (ACC: is_accessing e = Some (l, c)), loc_at l>>) /\
+        (<<CONT: nomix lang st1>>)
+  .
+
+  Definition nomix := paco2 _nomix bot2.
+  Arguments nomix: clear implicits.
+
+  Lemma nomix_mon: monotone2 _nomix.
+  Proof.
+    ii. exploit IN; eauto. i. des. splits.
+    { i. hexploit NA; eauto. }
+    { i. hexploit AT; eauto. }
+    { auto. }
+  Qed.
+  #[local] Hint Resolve nomix_mon: paco.
+End NOMIX.
+
+#[export] Hint Resolve nomix_mon: paco.
